%vec
\documentclass[10pt]{article}
\usepackage{pstricks}
\usepackage{pst-plot}
\usepackage{pst-node}
\usepackage{pst-tree}
\usepackage{pst-coil}

\usepackage[absolute]{textpos}
\setlength{\parindent}{0pt}
\usepackage{color}
\usepackage{amssymb}
\usepackage{graphicx}
\textblockorigin{0.5in}{0.5in}
\definecolor{MintGreen}      {rgb}{0.2,0.85,0.5}
\definecolor{LightGreen}     {rgb}{0.9,1,0.9}
\definecolor{LightYellow}    {rgb}{1,1,0.6}
\definecolor{test}           {rgb}{0.8,0.95,0.95}

\usepackage{hyperref}

\TPshowboxestrue
\TPMargin{2mm}
\begin{document}


\include{eucl_geo_anal}
\include{integral}
\include{complex}
\include{fourier}
\include{diff_forms_classical_vec}
\include{class_mech}
\include{em}

\null

\[
  \frac{d}{d t} {\mathbf S}_\phi = {\mathbf F}_\phi \left( {\mathbf S}_{\phi} ; t \right)
\]
\[
  \frac{d}{d t} {\mathbf S}_\eta = {\mathbf F}_\eta \left( {\mathbf S}_\eta ; t \right)
\]
\[
  \frac{d}{d t} {\mathbf T}_\phi = {\mathbf F}_\phi \left( {\mathbf T}_\phi ; t \right)
\]
\[
  \frac{d}{d t} {\mathbf T}_\eta = {\mathbf F}_\eta \left( {\mathbf T}_\eta ; t \right)
\]

\[
  \theta(x - q) = \left\{ \begin{array}{ll} 0 & x < q \\ 1 & x > q \end{array} \right.
\]
\[
 \int_{a}^{b} dx \, \theta(x-q) = \int_{a}^{q} d x
\]
\begin{eqnarray*}
 \int_{a}^{b} dx \, \theta(q - x)	& = & \int_{a}^{b} dx \left\{1 - \theta(x-q) \right\} \\
								& = & \int_{a}^{b} dx - \int_{a}^{q} dx \\
								& = & \int_{a}^{q} dx + \int_{q}^{b} dx - \int_{a}^{q} dx\\
								& = & \int_{q}^{b} dx
\end{eqnarray*}


\newpage
\null

Define an integrand
\[
  L(a,b)[f] = a f(x)^2 + b f'(x)^2
\]

\[
  I_v(a,b)[f] = \int_0^1 L(a,b)[f] dx = \int_0^1 \left( a f(x)^2 + b f'(x)^2 \right) dx
\]

\begin{tabular}{cc}
  $I_p(1,1)\left[x\right]$   & 1.33333 \\
  $I_p(1,1)\left[x^2\right]$ & 1.53333 \\
  $I_p(1,1)\left[x^3\right]$ & 1.94286
\end{tabular}
subject to the boundary conditions $f(0) = 0$ and $f(1) = 1$.
$I_p$ has as its domain any well-behaved function that is continuous and differentiable (this may be 
too restrictive).  Let the set of such functions be called $\mathcal D$.  Then let $\mathcal D'$ be
the subset of $\mathcal D$ that satisfies the boundary conditions.  Examples of $\mathcal D$ are:
$const, 0, \cos(x), x, x^2, (1-x^3), ln(x), \sin \left( \frac{\pi}{2} x \right), e^x$.  Examples
of $\mathcal D'$ are: $x, x^2, \sin \left( \frac{\pi}{2} \right)$.  


The goal is to find
$q \backepsilon {\mathcal D'}$ extremizes $I_p(a,b)[f]$ by taking the variation $\delta I_p$
and solve for $f$
\[
  \delta I_p = 2 \int_0^1 d\,x \left( a f \delta f + b f' \delta f' \right)
\]
\normalsize
%\begin{figure}[htpb!]
%\centering
%\includegraphics[width=170mm,height=150mm]{var_1.eps}
%\scriptsize\caption{Blah Blag}\label{fig:erptsqfit}
%\end{figure}
\newpage

\[
  \theta(x - q) = \left\{ \begin{array}{ll} 0 & x < q \\ 1 & x > q \end{array} \right.
\]
\[
 \int_{a}^{b} dx \, \theta(x-q) = \int_{a}^{q} d x
\]
\begin{eqnarray*}
 \int_{a}^{b} dx \, \theta(q - x)	& = & \int_{a}^{b} dx \left\{1 - \theta(x-q) \right\} \\
								& = & \int_{a}^{b} dx - \int_{a}^{q} dx \\
								& = & \int_{a}^{q} dx + \int_{q}^{b} dx - \int_{a}^{q} dx\\
								& = & \int_{q}^{b} dx
\end{eqnarray*}

$\bullet$  


\newpage
\null

%%%%%%%%%%%%%%%%%%%%%%%%%%%%%%%%%%%%%%%%%%%%%%%%%%%%%%%%%%%%%%%%%%%%%%%%%%%%%%%
%          Fourier Analysis
%%%%%%%%%%%%%%%%%%%%%%%%%%%%%%%%%%%%%%%%%%%%%%%%%%%%%%%%%%%%%%%%%%%%%%%%%%%%%%%
\textblockcolor{test}
\begin{textblock*}{7.5in}(0mm,0mm)
\begin{tabular*}{7.5in}{c @{\extracolsep{\fill}} c }
       \tiny ~ & ~\\
       \multicolumn{2}{c}{\normalsize \bf Periodic Functions, Fourier Analysis, and Sturm-Liouville Theory} \\
       \tiny~ & ~\\
\end{tabular*}
\end{textblock*}

\begin{textblock*}{90mm}(0mm,15mm)
Consider a periodic function $f(x-2\ell) = f(x) = f(x + 2\ell)$ defined on the interval $[-\ell,\ell]$.  
Because of the underlying periodicity of $f(x)$, both the derivative and the integral also inherit 
periodic properties.

In the case of the derivative, the observation is evident simply from 
the standard definition as follows:
\begin{eqnarray*}
  \frac{d f}{d x}(x) & = & \lim_{dx \rightarrow 0} \frac{ f(x+dx)-f(x)}{dx}\\
                     & = & \lim_{dx \rightarrow 0} \frac{ f(x + 2\ell + dx) - f(x + 2\ell) }{dx} \\
                     & = & \frac{d f}{d x}(x + 2\ell).
\end{eqnarray*}
In the case of the integral, a bit more thinking and manipulation is needed.
To begin, consider the integral of $f(x)$ over an interval $[a,b]$.  The value of this integral 
is invariant if the entire interval is shifted by $2 \ell$.  This is proven by direct substitution
as 
\begin{eqnarray}\label{eq_per_ab_int}
  \int_{a}^{b} f(x) dx & = & \int_{a}      ^{b}       f(x - 2\ell) dx            \\
                       & = & \int_{a+2\ell}^{b+2\ell} f(y)         dy  \nonumber \\
                       & = & \int_{a+2\ell}^{b+2\ell} f(x)         dx. \nonumber
\end{eqnarray}
With this result, it is easy (although somewhat subtle) to show that the integral
of $f(x)$ over the interval $[c-\ell,c+\ell]$ is equal to the integral over 
the interval $[-\ell,\ell]$.  To do so, start by letting $a = c - \ell$ and $b = -\ell$
in (\ref{eq_per_ab_int}), which yields the identity 
\begin{equation}\label{eq_per_int}
  \int_{c-\ell}^{-\ell} f(x) dx  =  \int_{c+\ell}^{\ell} f(x) dx,
\end{equation}
which is then used to manipulate the integral over $[c-\ell,c+\ell]$ as follows,
\begin{eqnarray} 
  \int_{c-\ell}^{c+\ell} f(x) dx  & = &  \int_{c-\ell}^{-\ell} f(x) dx + \int_{-\ell}^{c+\ell} f(x) dx \\
                                  & = &  \int_{c+\ell}^{\ell}  f(x) dx + \int_{-\ell}^{c+\ell} f(x) dx \nonumber \\
                                  & = &  \int_{-\ell}^{c+\ell} f(x) dx + \int_{c+\ell}^{\ell}  f(x) dx \nonumber \\
                                  & = &  \int_{-\ell}^{\ell}   f(x) dx                                 \nonumber
\end{eqnarray}
where (\ref{eq_per_int}) was used in going from the first to the second line.

\[
  -\frac{d}{d x}\left( p(x) \frac{d y}{d x} \right) + q(x) y = \lambda w(x) y
\]
\end{textblock*}

\begin{textblock*}{100mm}(89.85mm,15mm)
\[
  \int_{c}^{c+2L} \cos \left( \frac{m \pi x}{L} \right) dx = 0
 \]
 \[
  \int_{c}^{c+2L} \sin \left( \frac{m \pi x}{L} \right) dx = 0
 \]
 
\[
  \int_{c}^{c+2L} dx \, \cos \left( \frac{m \pi x}{L} \right) \cos \left( \frac{n \pi x}{L} \right) = 
      \left\{ \begin{array}{cc} 2 L \, \delta_{mn} & m = 0 \\ L \, \delta_{mn} & m \neq 0 \end{array} \right.
\]
\[
  \int_{c}^{c+2L} dx \, \sin \left( \frac{m \pi x}{L} \right) \sin \left( \frac{n \pi x}{L} \right) = 
      \left\{ \begin{array}{cc} 0 \, \delta_{mn} & m = 0 \\ L \, \delta_{mn} & m \neq 0 \end{array} \right.
\]
\[
 {\tilde f}(x) = \frac{a_0}{2} + 
    \sum_{n=1}^{\infty} \left( a_n \cos \left( \frac{n \pi x}{L} \right) + b_n \sin \left( \frac{n \pi x}{L} \right) \right)
\]
\[
  a_n = \frac{1}{L} \int_{c}^{c+2L} f(x) \cos \left( \frac{n \pi x}{L} \right) dx
\]
\[
  b_n = \frac{1}{L} \int_{c}^{c+2L} f(x) \sin \left( \frac{n \pi x}{L} \right) dx
\]

\[
  {\tilde f}(x) = \sum_{n = - \infty}^{\infty} c_n e^{i n \pi x/L}
\]
\[
  c_n = \frac{1}{2 L} \int_{c}^{c+2L} f(x) e^{-i n \pi x/L} dx
\]
\end{textblock*}
\newpage
\null
%%%%%%%%%%%%%%%%%%%%%%%%%%%%%%%%%%%%%%%%%%%%%%%%%%%%%%%%%%%%%%%
%          Harmonic Oscillators
%%%%%%%%%%%%%%%%%%%%%%%%%%%%%%%%%%%%%%%%%%%%%%%%%%%%%%%%%%%%%%%
\textblockcolor{test}
\begin{textblock*}{7.5in}(0mm,0mm)
\begin{tabular*}{7.5in}{c @{\extracolsep{\fill}} c }
       \tiny ~ & ~\\
       \multicolumn{2}{c}{\normalsize \bf Harmonic Oscillators} \\
       \tiny~ & ~\\
\end{tabular*}
\end{textblock*}

\begin{textblock*}{2.5in}(0mm,30mm)
The equation for a damped simple harmonic oscillator is
\[
  m {\ddot x} + \Gamma {\dot x} + k x = 0 .
\]
Assume a solution of the form $x = A e^{\imath \omega t}$ and then substitute into the equation of motion.
Factoring out $A e^{i \omega t}$, yields the characteristic equation
\[
  -m \omega^2 + i \Gamma \omega + k = 0 .
\]
Before solving the charateristic equation, divide by $m$ and then define the parameters ${\omega_0}^2 = k/m$ and 
$\gamma = \Gamma/2$.  The equation then becomes
\[
  \omega^2 - i \gamma \omega + {\omega_0}^2 = 0
\]
with corresponding roots
\[
  \omega = \frac{i \gamma}{2} \pm \sqrt{ {\omega_0}^2 - \frac{\gamma^2}{4} } 
         = \frac{i \gamma}{2} \pm \omega_D
\]
Thus the final solution looks like
\[
  x = e^{-i \gamma/2} \left[ x_0 \cos(\omega_D t) + \frac{v_0}{\omega_D} \sin(\omega_D t) \right]
\]
\end{textblock*}
\newpage
\null

\end{document} 